AwsCryptographicMaterialProviders/dafny/AwsCryptographyKeyStoreAdmin/src/KeyStoreAdminErrorMessages.dfy
@@ -5,6 +5,9 @@ module {:options "/functionSyntax:4" } KeyStoreAdminErrorMessages {
   const NO_MUTATE_TO_HV_1: string :=
     "At this time, a Mutation cannot change a Branch Key from HV-2 to HV-1. The request dictated 'TerminalHierarchyVersion := v1' and was therefore rejected. Remove the 'TerminalHierarchyVersion' parameter or set it to at least 'v2'."
 
-  const UNSUPPORTED_KEYMANAGEMENTSTRATEGY_HV_2: string :=
-    "Only KeyManagementStrategy.AwsKmsSimple is allowed when mutating to hv-2."
+  const UNSUPPORTED_KEYMANAGEMENTSTRATEGY :=
+    "Unsupported KeyManagementStrategy."
+    + " Only KeyManagementStrategy.AwsKmsReEncrypt and KeyManagementStrategy.AwsKmsDecryptEncrypt"
+    + " is allowed when terminal hierarchical version is 1."
+    + " Only KeyManagementStrategy.kmsSimple is allowed when terminal hierarchical version is 2."
 }
